$$ \mu = \frac{1}{\sin^{-1}(M)} $$

$$
\nu = \sqrt{\frac{\gamma + 1}{\gamma - 1}} \cdot \tan^{-1}\left( \sqrt{\frac{\gamma - 1}{\gamma + 1} (M^2 - 1) } \right)
    - \tan^{-1}\left( \sqrt{ (M^2 - 1) } \right)
$$

$$
\frac{p}{p_0} = \left( 1 + \frac{\gamma - 1}{2} M^2 \right) ^ {-\frac{\gamma}{\gamma - 1}}
$$

$$
\frac{\rho}{\rho_0} = \left( 1 + \frac{\gamma - 1}{2} M^2 \right) ^ {-\frac{1}{\gamma - 1}}
$$

$$
\frac{T}{T_0} = \left( 1 + \frac{\gamma - 1}{2} M^2 \right) ^ {-1}
$$

$$
\frac{p}{p^*} = \left( \frac{2 + (\gamma - 1) M^2}{\gamma + 1} \right) ^ {-\frac{\gamma}{\gamma - 1}}
$$

$$
\frac{\rho}{\rho^*} = \left( \frac{2 + (\gamma - 1) M^2}{\gamma + 1} \right) ^ {-\frac{1}{\gamma - 1}}
$$

$$
\frac{T}{T^*} = \frac{\gamma + 1}{2 + (\gamma - 1) M^2}
$$

$$
\frac{A}{A^*} = \left( \frac{\gamma + 1}{2} \right) ^ {-\frac{\gamma + 1}{2(\gamma - 1)}}
          \cdot \left( \frac{1 + \frac{\gamma - 1}{2} M^2}{M} \right) ^ {\frac{\gamma + 1}{2(\gamma - 1)}}
$$